#+TITLE: Practice 17

#+BEGIN_EXAMPLE

if (test-expr) {
    then-statement
} else {
    else-statement
}


# case 1
t = test-expr
if (!t) {
    goto false;
}
then-statement
goto done;

false:
    else-statement
done:


# case 2
t = test-expr
if (t) {
    goto true;
}
else-statement
goto done;

true:
    then-statement
done:

#+END_EXAMPLE

#+BEGIN_SRC c

long lt_cnt = 0;
long ge_cnt = 0;

long abs_diff_se(long x, long y)
{
    long result;
    if (x < y) {
        lt_cnt++;
        result = y - x;
    } else {
        ge_cnt++;
        result = x - y;
    }
    return result;
}

#+END_SRC


#+BEGIN_SRC c

/* case 1 */
long lt_cnt = 0;
long ge_cnt = 0;

long abs_diff_se(long x, long y)
{
    long result;
    if (x >= y) {
        goto x_ge_y;
    }

    lt_cnt++;
    result = y - x;
    return result;

x_ge_y:
    ge_cnt++;
    result = x - y;
    return result;
}

#+END_SRC


#+BEGIN_SRC c

/* case 2 */
long lt_cnt = 0;
long ge_cnt = 0;

long abs_diff_se(long x, long y)
{
    long result;
    if (x < y) {
        goto x_lt_y;
    }

    ge_cnt++;
    result = x - y;
    result result;

x_lt_y:
    lt_cnt++;
    result = y - x;
    return result;
}

#+END_SRC

*if non else-statement case 1 is fine, otherwise same*
