#+AUTHOR: Fei Li
#+EMAIL: wizard@pursuetao.com
* Practice 85
  
  #+BEGIN_EXAMPLE
  E    k-bit
  M    n-bit
  #+END_EXAMPLE

** A  

   {0} {100...001} {1100...00}

   M = 1 + 3/4 = 7/4
   E = bias+2 - bias = 2
   V = 2^E * M = 2^2 * 7/4 = 7


** B

   {0} {bias+n} {11...11}
   
   M = 2 - 2^-n
   V = M * 2^E = (2 - 2^-n) * 2^(bias+n - bias) = 2^(n+1) - 1


** C
   
   {0} {11...11 01} {00...00}

   M = 1
   E = 2 * bias - 1
   V = 2^E * M = 2^E = 2^(2*bias-1 - bias) = 2^(bias - 1)

   V(-1) = 2^(1 - bias)
